gate ordinary checker by safety routes

fixtures/TypeChecker.ml
@@ -6038,32 +6038,6 @@ let infer_program_env_alpha_elab env =
        env_alpha.env_traits; env_impls = env_alpha.env_impls; env_fns = fns' }
    | Infer_err err -> Infer_err err)
 
-(** val check_program_env : global_env -> bool **)
-
-let check_program_env env =
-  forallb (fun f ->
-    match infer_full_env env f with
-    | Infer_ok _ -> true
-    | Infer_err _ -> false) env.env_fns
-
-(** val check_program_env_alpha : global_env -> bool **)
-
-let check_program_env_alpha env =
-  check_program_env (alpha_normalize_global_env env)
-
-(** val check_program_env_alpha_validated : global_env -> bool **)
-
-let check_program_env_alpha_validated env =
-  (&&) (top_level_names_unique_b (alpha_normalize_global_env env))
-    (check_program_env_alpha env)
-
-(** val check_program_env_alpha_elab : global_env -> bool **)
-
-let check_program_env_alpha_elab env =
-  match infer_program_env_alpha_elab env with
-  | Infer_ok _ -> true
-  | Infer_err _ -> false
-
 (** val fn_params_roots_exclude_b : param list -> root_set -> bool **)
 
 let fn_params_roots_exclude_b ps roots =
@@ -6566,6 +6540,42 @@ let check_env_root_shadow_direct_call_provenance_summary env =
 let check_env_root_shadow_captured_call_provenance_summary env =
   forallb (check_fn_root_shadow_captured_call_provenance_summary env)
     env.env_fns
+
+(** val check_fn_ordinary_safety_gate : global_env -> fn_def -> bool **)
+
+let check_fn_ordinary_safety_gate env fdef =
+  (||)
+    ((||)
+      ((||) (check_fn_root_shadow_summary env fdef)
+        (check_fn_root_shadow_direct_call_provenance_summary env fdef))
+      (check_fn_root_shadow_non_capturing_call_provenance_summary env fdef))
+    (check_fn_root_shadow_captured_call_provenance_summary env fdef)
+
+(** val check_program_env : global_env -> bool **)
+
+let check_program_env env =
+  forallb (fun f ->
+    match infer_full_env env f with
+    | Infer_ok _ -> check_fn_ordinary_safety_gate env f
+    | Infer_err _ -> false) env.env_fns
+
+(** val check_program_env_alpha : global_env -> bool **)
+
+let check_program_env_alpha env =
+  check_program_env (alpha_normalize_global_env env)
+
+(** val check_program_env_alpha_validated : global_env -> bool **)
+
+let check_program_env_alpha_validated env =
+  (&&) (top_level_names_unique_b (alpha_normalize_global_env env))
+    (check_program_env_alpha env)
+
+(** val check_program_env_alpha_elab : global_env -> bool **)
+
+let check_program_env_alpha_elab env =
+  match infer_program_env_alpha_elab env with
+  | Infer_ok env' -> check_program_env env'
+  | Infer_err _ -> false
 
 (** val check_env_preservation_ready : global_env -> bool **)
 
